Different induction for arity analysis improvement lemma

Launchbury/ArityAnalysis.thy
@@ -16,24 +16,33 @@ lemma Aexp'_simps[simp]:
   "Aexp' e \<cdot> (up\<cdot>n) = Aexp e \<cdot> n"
   unfolding Aexp'_def by simp_all
 
-definition AE_singleton :: "var \<Rightarrow> Arity\<^sub>\<bottom> \<Rightarrow> AEnv"
-  where "AE_singleton x a y = (if x = y then a else \<bottom>)"
+definition AE_singleton :: "var \<Rightarrow> Arity\<^sub>\<bottom> \<rightarrow> AEnv"
+  where "AE_singleton x = (\<Lambda> a. (\<lambda> y . (if x = y then a else \<bottom>)))"
 
-lemma AE_singleton_bot[simp]: "AE_singleton x \<bottom> = \<bottom>"
+lemma AE_singleton_bot[simp]: "AE_singleton x \<cdot> \<bottom> = \<bottom>"
   by (rule ext)(simp add: AE_singleton_def)
+
+lemma AE_singleton_simps[simp]: "(AE_singleton x \<cdot> n) x = n"
+  by (simp add: AE_singleton_def)
 
 lemma up_zero_top[simp]: "x \<sqsubseteq> up\<cdot>(0::Arity)"
   by (cases x) auto
 
-lemma AE_singleton_below_iff[simp]: "AE_singleton x a \<sqsubseteq> ae  \<longleftrightarrow> a \<sqsubseteq> ae x"
+lemma AE_singleton_below_iff[simp]: "AE_singleton x \<cdot> a \<sqsubseteq> ae  \<longleftrightarrow> a \<sqsubseteq> ae x"
   by (auto simp add: fun_below_iff AE_singleton_def)
 
 definition ABind :: "var \<Rightarrow> exp \<Rightarrow> (AEnv \<rightarrow> AEnv)"
   where "ABind v e = (\<Lambda> ae. Aexp' e \<cdot> (ae v))"
 
+lemma ABind_eq[simp]: "ABind v e \<cdot> ae = Aexp' e \<cdot> (ae v)"
+  unfolding ABind_def by (simp add: cont_fun)
+
 fun ABinds :: "heap \<Rightarrow> (AEnv \<rightarrow> AEnv)"
   where "ABinds [] = ID"
      |  "ABinds ((v,e)#binds) = ABind v e \<squnion> ABinds (delete v binds)"
+
+lemma ABinds_strict[simp]: "ABinds \<Gamma>\<cdot>\<bottom>=\<bottom>"
+  by (induct \<Gamma> rule: ABinds.induct) auto
 
 lemma Abinds_reorder1: "map_of \<Gamma> v = Some e \<Longrightarrow> ABinds \<Gamma> = ABind v e \<squnion> ABinds (delete v \<Gamma>)"
 proof (induction \<Gamma> rule: ABinds.induct)
@@ -64,7 +73,6 @@ next
   show ?case by auto
 qed
 
-
 lemma ABinds_above_arg: "ae \<sqsubseteq> ABinds \<Gamma> \<cdot> ae"
 proof (induction rule:ABinds.induct)
   show "ae \<sqsubseteq> ABinds []\<cdot>ae" by auto
@@ -80,6 +88,43 @@ definition Afix ::  "heap \<Rightarrow> (AEnv \<rightarrow> AEnv) \<rightarrow> 
 
 lemma Afix_eq: "Afix \<Gamma> \<cdot> F \<cdot> ae = (\<mu>  ae'. ae \<squnion> ((ABinds \<Gamma> \<cdot> ae') \<squnion> F \<cdot> ae'))"
   unfolding Afix_def by simp
+
+definition Afix2 ::  "heap \<Rightarrow> (AEnv \<rightarrow> AEnv)"
+  where "Afix2 \<Gamma> = (\<Lambda> ae. (\<mu>  ae'. ABinds \<Gamma> \<cdot> ae' \<squnion> ae))"
+
+lemma Afix2_eq: "Afix2 \<Gamma> \<cdot> ae = (\<mu>  ae'. (ABinds \<Gamma> \<cdot> ae') \<squnion> ae)"
+  unfolding Afix2_def by simp
+
+lemma Afix2_strict[simp]: "Afix2 \<Gamma> \<cdot> \<bottom> = \<bottom>"
+  unfolding Afix2_eq
+  by (rule fix_eqI) auto
+
+lemma Afix2_least_below: "ABinds \<Gamma> \<cdot> ae' \<sqsubseteq> ae' \<Longrightarrow> ae \<sqsubseteq> ae' \<Longrightarrow> Afix2 \<Gamma> \<cdot> ae \<sqsubseteq> ae'"
+  unfolding Afix2_eq
+  by (auto intro: fix_least_below)
+
+lemma Abinds_below_Afix2: "ABinds \<Delta> \<sqsubseteq> Afix2 \<Delta>"
+  apply (rule cfun_belowI)
+  apply (simp add: Afix2_eq)
+  apply (subst fix_eq, simp)
+  apply (rule below_trans[OF _ join_above1])
+  apply (rule monofun_cfun_arg)
+  apply (subst fix_eq, simp)
+  done
+
+lemma Afix2_above_arg: "ae \<sqsubseteq> Afix2 \<Gamma> \<cdot> ae"
+  by (metis (hide_lams, no_types) Abinds_below_Afix2 ArityAnalysis.ABinds_above_arg below_refl box_below monofun_cfun_fun)
+
+lemma join_self_below[iff]:
+  "x = x \<squnion> y \<longleftrightarrow> y \<sqsubseteq> (x::'a::Finite_Join_cpo)"
+  by (metis "HOLCF-Join-Classes.join_above2" larger_is_join1)
+
+lemma Abinds_Afix[simp]: "ABinds \<Gamma>\<cdot>(Afix2 \<Gamma>\<cdot>ae) = Afix2 \<Gamma>\<cdot>ae"
+  unfolding Afix2_eq
+  apply (subst fix_eq) back apply simp
+  apply (rule below_trans[OF ABinds_above_arg monofun_cfun_arg])
+  apply (subst fix_eq) apply simp
+  done
 
 definition Acomplete :: "heap \<Rightarrow> exp \<Rightarrow> (AEnv \<rightarrow> AEnv) \<Rightarrow> Arity \<rightarrow> AEnv"
   where "Acomplete \<Gamma> e F = (\<Lambda> a. (\<mu> ae. ABinds \<Gamma> \<squnion> F) \<cdot> (Aexp e \<cdot> a))"
